@prefix owl: <http://www.w3.org/2002/07/owl#> .
@prefix rdf: <http://www.w3.org/1999/02/22-rdf-syntax-ns#> .
@prefix rdfs: <http://www.w3.org/2000/01/rdf-schema#> .
@prefix dct: <http://purl.org/dc/terms/> .
@prefix schema: <http://schema.org/> .
@prefix dbpedia: <http://dbpedia.org/resource/> .
@prefix ifx: <np00.github.io/ifxProductOntology.html#> . #dummy
@prefix xsd: <http://www.w3.org/2001/XMLSchema#> .
@prefix foaf: <http://xmlns.com/foaf/0.1/> .


# Description of this ontology
# ----------------------------

ifx: a owl:Ontology ;
    dct:title "The Infineon Product Ontology"@en;
    rdfs:comment "The Infineon Product Ontology provides a unique namespace and description for Infineon Products in a machine-readable format. The information is derived from the official Infineon <a href=\"http://www.infineon.com/cms/en/product/power/mosfet/small-signal-mosfet/20v-800v-n-channel-and-p-channel-small-signal-mosfet/channel.html?channel=ff80808112ab681d0112ab6a590004ba\">product catalog</a>. The documentation was generated using  <a href=\"http://www.essepuntato.it/lode\">LODE</a>";
    dct:creator "Niklas Petersen" ; 
    dct:publisher "Fraunhofer IAIS";
    dct:date "2017-01-31";
    owl:versionInfo "0.0.1".

ifx:Transistor
	a rdfs:Class , owl:Class ;
	rdfs:comment "The metal–oxide–semiconductor field-effect transistor (MOSFET, MOS-FET, or MOS FET) is a type of field-effect transistor (FET). It has an insulated gate, whose voltage determines the conductivity of the device." ;
	rdfs:isDefinedBy <https://en.wikipedia.org/wiki/MOSFET> ;
	rdfs:label "Transistor"@en , "Transistor"@de .

# Properties

ifx:opn
	a owl:DatatypeProperty ; 
	rdfs:comment "Describes the OPN of a Transistor." ; 
	rdfs:label "OPN"@en , "OPN"@de ;
	rdfs:domain ifx:Transistor ;
	rdfs:range xsd:string .

ifx:package
	a owl:DatatypeProperty ; 
	rdfs:comment "Describes the package of a transistor." ; 
	rdfs:label "Package"@en , "Package"@de ;
	rdfs:domain ifx:Transistor ;
	rdfs:range xsd:string .

ifx:transistorTechnology
	a owl:DatatypeProperty ; 
	rdfs:comment "Describes the technology of a transistor." ; 
	rdfs:label "Transistor Technology"@en , "Transistor Technology"@de ;
	rdfs:domain ifx:Transistor ;
	rdfs:range xsd:string .
	
ifx:priceInEuroPer1k
	a rdf:Property , owl:DatatypeProperty ; 
	rdfs:comment "Defined price for a product for a volume of 1.000 units." ; 
	rdfs:label "Price for an order of 1,000 units."@en , "Preis für eine Bestellung von 1,000 Einheiten"@de ;
	rdfs:domain schema:Product ;
	rdfs:range xsd:decimal .
	

schema:manufacturer a rdf:Property ;
	rdfs:label "manufacturer" ; 
	rdfs:comment "The manufacturer of the product." ;
	rdfs:domain schema:Product ; 
	. 

dbpedia:Infineon_Technologies rdf:type dbpedia:Organisation ;
	rdfs:label	"Infineon Technologies"@de , "Infineon Technologies"@en ;
	rdfs:comment "Infineon Technologies AG is a German semiconductor manufacturer founded on 1 April 1999, when the semiconductor operations of the parent company Siemens AG were spun off to form a separate legal entity. As of 30 September 2013, Infineon has 26,725 employees worldwide. In fiscal year 2013, the company achieved sales of \u20AC3.843 billion.On 1 May 2006, Infineon's Memory Products division was carved out as a distinct company called Qimonda AG, which at its height employed about 13,500 people worldwide. Qimonda was listed on the New York Stock Exchange until 2009."@en ;
	foaf:homepage	<https://www.infineon.com/> ;
	.


	
# Individuals	
	
ifx:BSR202N   
	schema:name "BSR202N" ;
	schema:manufacturer dbpedia:Infineon_Technologies ;
	ifx:opn "BSR202NL6327HTSA1" ;
	ifx:package "SC59" ;
	ifx:transistorTechnology "OptiMOS 2";
	ifx:priceInEuroPer1k 0.09 ;
	.

ifx:IRLL3303      
	schema:name "IRLL3303" ;
	schema:manufacturer dbpedia:Infineon_Technologies ;
	ifx:opn "IRLL3303TRPBF" ;
	ifx:package "SOT-223" ;
	ifx:transistorTechnology "Planar Mosfet" ;
	ifx:priceInEuroPer1k 0.27 ;
	.

ifx:BSP295      
	schema:name "BSP295" ;
	schema:manufacturer dbpedia:Infineon_Technologies ;
	ifx:opn "BSP295H6327XTSA1" ;
	ifx:package "SOT-223" ;
	ifx:transistorTechnology "SIPMOS";
	ifx:priceInEuroPer1k 0.17 ;
	.

ifx:BSL306N      
	schema:name "BSL306N" ;
	schema:manufacturer dbpedia:Infineon_Technologies ;
	ifx:opn "BSL306NH6327XTSA1" ;
	ifx:package "TSOP-6 dual" ;
	ifx:transistorTechnology "OptiMOS 2" ;
	ifx:priceInEuroPer1k 0.09 ;
	.